src/MinimalLogging.v
@@ -1,6 +1,6 @@
 Require Import Coq.ZArith.BinInt.
 Require Import riscv.util.BitWidths.
-Require Import riscv.util.Monads.
+Require Import riscv.util.Monads. Import OStateOperations.
 Require Import riscv.Decode.
 Require Import riscv.Memory. (* should go before Program because both define loadByte etc *)
 Require Import riscv.Program.
